LinearScan/Lib.hs
@@ -46,6 +46,16 @@ foldl_with_index f b v =
       (:) y ys -> go ((Prelude.succ) n) ys (f n z y)}}
   in go 0 v b
 
+mapAccumL :: (a1 -> a2 -> (,) a1 a3) -> a1 -> ([] a2) -> (,) a1 ([] a3)
+mapAccumL f s v =
+  case v of {
+   [] -> (,) s [];
+   (:) x xs ->
+    case f s x of {
+     (,) s' y ->
+      case mapAccumL f s' xs of {
+       (,) s'' ys -> (,) s'' ((:) y ys)}}}
+
 dep_foldl_inv :: (a1 -> Eqtype.Equality__Coq_type) -> a1 -> ([]
                  Eqtype.Equality__Coq_sort) -> Prelude.Int -> (a1 -> []
                  Eqtype.Equality__Coq_sort) -> (a1 -> a1 -> () ->
