LinearScan/seq.hs
@@ -12,6 +12,7 @@ import qualified LinearScan.Utils
 
 import qualified LinearScan.Eqtype as Eqtype
 import qualified LinearScan.Ssrbool as Ssrbool
+import qualified LinearScan.Ssrnat as Ssrnat
 
 
 
@@ -24,6 +25,38 @@ unsafeCoerce = GHC.Base.unsafeCoerce#
 import qualified LinearScan.IOExts as IOExts
 unsafeCoerce = IOExts.unsafeCoerce
 #endif
+
+ncons :: Prelude.Int -> a1 -> ([] a1) -> [] a1
+ncons n x =
+  Ssrnat.iter n (\x0 -> (:) x x0)
+
+nseq :: Prelude.Int -> a1 -> [] a1
+nseq n x =
+  ncons n x []
+
+nth :: a1 -> ([] a1) -> Prelude.Int -> a1
+nth x0 s n =
+  case s of {
+   [] -> x0;
+   (:) x s' ->
+    (\fO fS n -> if n Prelude.== 0 then fO () else fS (n Prelude.- 1))
+      (\_ ->
+      x)
+      (\n' ->
+      nth x0 s' n')
+      n}
+
+set_nth :: a1 -> ([] a1) -> Prelude.Int -> a1 -> [] a1
+set_nth x0 s n y =
+  case s of {
+   [] -> ncons n x0 ((:) y []);
+   (:) x s' ->
+    (\fO fS n -> if n Prelude.== 0 then fO () else fS (n Prelude.- 1))
+      (\_ -> (:) y
+      s')
+      (\n' -> (:) x
+      (set_nth x0 s' n' y))
+      n}
 
 catrev :: ([] a1) -> ([] a1) -> [] a1
 catrev s1 s2 =
